\documentclass{jsarticle}
\usepackage{tensor}
\usepackage{amsmath}
\usepackage{mathtools}

\title{Schwartzschild 解のRicci テンソル}
\author{}

\begin{document}
    \maketitle

%\begin{equation}
%    \tensor{g}{_{\mu\nu}} = 
%    \left\{ \
%        \begin{aligned}
%            &\tensor{g}{_{00}} = -e^{\nu(r)}\\
%            &\tensor{g}{_{11}} = r^2\\
%            &\tensor{g}{_{22}} = r^2\sin\theta\\
%            &\tensor{g}{_{33}} = e^{\lambda(r)}
%        \end{aligned}
%    \right.
%    , \quad
%    \tensor{g}{^{\mu\nu}}
%    \left\{ \
%        \begin{aligned}
%            &\tensor{g}{^{00}} = -e^{-\nu(r)}\\
%            &\tensor{g}{^{11}} = r^{-2}\\
%            &\tensor{g}{^{22}} = (r^2\sin\theta)^{-1}\\
%            &\tensor{g}{^{33}} = e^{-\lambda(r)}
%        \end{aligned}
%    \right.
%\end{equation}

\begin{equation}
   \tensor{\varGamma}{^\rho_{\mu\nu}} = 
    \left\{  \
        \begin{aligned}
            &\tensor{\varGamma}{^0_{03}} = \tensor{\varGamma}{^0_{30}} = \frac{1}{2} \nu'\\
            &\tensor{\varGamma}{^1_{13}} = \tensor{\varGamma}{^1_{31}} = r^{-1}\\
            &\tensor{\varGamma}{^2_{12}} = \tensor{\varGamma}{^1_{21}} = \cot\theta\\
            &\tensor{\varGamma}{^2_{23}} = \tensor{\varGamma}{^2_{32}} = r^{-1}\\
            &\tensor{\varGamma}{^3_{00}} = -\frac{1}{2} \nu'e^{-\lambda + \nu}\\ 
            &\tensor{\varGamma}{^3_{11}} = -re^{-\lambda}\\
            &\tensor{\varGamma}{^3_{22}} = -re^{-\lambda}\sin^2\theta\\
            &\tensor{\varGamma}{^3_{33}} = \frac{1}{2} \lambda'
        \end{aligned}
    \right. 
\end{equation}

%Swartzschild の座標系における計量および Christoffel 記号は以上の通りである．ここで，Ricci テンソル
%を計算する．

\begin{equation}
    \tensor{R}{_{\mu\nu}} = \partial_\rho \tensor{\varGamma}{^\rho_{\mu\nu}} 
                            - \partial_\nu \tensor{\varGamma}{^\rho_{\mu\rho}}
                            + \tensor{\varGamma}{^\sigma_{\mu\nu}} \tensor{\varGamma}{^\rho_{\rho\sigma}}
                            - \tensor{\varGamma}{^\tau_{\mu\rho}} \tensor{\varGamma}{^\rho_{\nu\tau}}
\end{equation}

\begin{align}
    \tensor{R}{_{33}} &= \underbrace{\partial_\rho \tensor{\varGamma}{^\rho_{33}}}_{\rho=3} 
                            - \underbrace{\partial_3 \tensor{\varGamma}{^\rho_{3\rho}}}_{\rho=0,1,2,3}
                            + \underbrace{\tensor{\varGamma}{^\sigma_{33}} \tensor{\varGamma}{^\rho_{\rho\sigma}}}_{\sigma=3,\rho=0,1,2,3}
                            - \underbrace{\tensor{\varGamma}{^\tau_{3\rho}} \tensor{\varGamma}{^\rho_{3\tau}}}_{\tau=\rho=0,1,2,3}\\\nonumber
    \\
    &= \begin{multlined}[t]
            \partial_3 \tensor{\varGamma}{^3_{33}}
            - \partial_3 \tensor{\varGamma}{^0_{30}} 
            - \partial_3 \tensor{\varGamma}{^1_{31}}
            - \partial_3 \tensor{\varGamma}{^2_{32}}
            - \partial_3 \tensor{\varGamma}{^3_{33}}\\
            + \tensor{\varGamma}{^3_{33}} \tensor{\varGamma}{^0_{03}}
            + \tensor{\varGamma}{^3_{33}} \tensor{\varGamma}{^1_{13}}
            + \tensor{\varGamma}{^3_{33}} \tensor{\varGamma}{^2_{23}}
            + \tensor{\varGamma}{^3_{33}} \tensor{\varGamma}{^3_{33}}\\
            - \tensor{\varGamma}{^0_{30}} \tensor{\varGamma}{^0_{30}}            
            - \tensor{\varGamma}{^1_{31}} \tensor{\varGamma}{^1_{31}}
            - \tensor{\varGamma}{^2_{32}} \tensor{\varGamma}{^2_{32}}
            - \tensor{\varGamma}{^3_{33}} \tensor{\varGamma}{^3_{33}}
        \end{multlined}\\\nonumber
        \\
    &= \begin{multlined}[t]
            - \partial_3 \tensor{\varGamma}{^0_{30}} 
            - \partial_3 \tensor{\varGamma}{^1_{31}}
            - \partial_3 \tensor{\varGamma}{^2_{32}}\\
            + \tensor{\varGamma}{^3_{33}} \tensor{\varGamma}{^0_{03}}
            + \tensor{\varGamma}{^3_{33}} \tensor{\varGamma}{^1_{13}}
            + \tensor{\varGamma}{^3_{33}} \tensor{\varGamma}{^2_{23}}\\
            - (\tensor{\varGamma}{^0_{30}})^2            
            - (\tensor{\varGamma}{^1_{31}})^2
            - (\tensor{\varGamma}{^2_{32}})^2 
        \end{multlined}\\\nonumber
        \\
    &= \begin{multlined}[t]
            - \frac{1}{2}\nu'' + r^{-1} + r^{-1}\\ 
            + \frac{1}{2}\lambda'\frac{1}{2}\nu' + \frac{1}{2}\lambda'r^{-1} + \frac{1}{2}\lambda'r^{-1}
            + \frac{1}{4}{\lambda'}^2\\
            - \frac{1}{4}{\nu'}^2 - r^{-2} - r^{-2} - \frac{1}{4}{\lambda'}^2
        \end{multlined}\\\nonumber
        \\
    &= \begin{multlined}[t]
            - \frac{1}{2}\nu''-\frac{1}{4}{\nu'}^2+\frac{1}{4}{\lambda'\nu'}+\frac{\lambda'}{r}
        \end{multlined}
\end{align}








\end{document}
